theories/FOL/ModelTheory/AnalysisLS.v
@@ -6,15 +6,15 @@ Require Import Undecidability.FOL.ModelTheory.Core.
 Section LSiffDC.
 
     Corollary LS_iff_DC_under_AC00_LEM: 
-        AC00 -> LEM -> DLS <-> DC.
+        CC_nat -> LEM -> DLS <-> DC.
     Proof.
         intros H1 H2; split.
         - eapply LS_CC_impl_DC; eauto.
-        - intros DC. eapply LS_correct, LS_downward_with_DC_LEM; eauto.
+        - intros DC. eapply LS_downward_with_DC_LEM; eauto.
     Qed.
 
     Corollary LS_iff_DC_BDP_BEP_under_AC00:
-        AC00 -> DLS <-> DC /\ BDP /\ BEP.
+        CC_nat -> DLS <-> DC /\ BDP /\ BEP.
     Proof.
         intros H1; split.
         - intros HLS. repeat split.
@@ -22,7 +22,7 @@ Section LSiffDC.
           now apply LS_impl_BDP.
           now apply LS_impl_BEP.
         - intros (h1 & h2 & h3).
-          now apply LS_correct, LS_downward_with_BDP_BEP_DC.
+          now apply LS_downward_with_BDP_BEP_DC.
     Qed.
 
     Corollary LS_iff_DDC_BDP_BEP_BCC:
@@ -31,12 +31,32 @@ Section LSiffDC.
         split.
         - intros HLS. repeat split.
           assert (OBDC) as HO. now  apply LS_impl_OBDC.
-          assert (BDC2) as H2. intros X. now apply OBDC_impl_BDC2_on.
+          assert (BDC2) as H2. intros X x. now apply OBDC_impl_BDC2_on, HO.
           now apply BDC2_iff_DDC_BCC.
           now apply LS_impl_BDP. now apply LS_impl_BEP.
           now eapply BDC_impl_BCC, LS_impl_BDC. 
         - intros (h1 & h2 & h3 & h4).
-          now apply LS_correct, LS_downward.
+          now apply  LS_downward.
     Qed.
+
+    Theorem Decomposition:
+      (DLS -> DDC /\ BDP /\ BEP /\ BCC) 
+        /\ 
+      (DDC /\ BDP /\ BEP /\ BCC -> BDP /\ BEP /\ BDC2) 
+        /\ 
+      (BDC2 /\ BDP /\ BEP -> OBDC) 
+        /\ 
+      (OBDC -> DLS).
+    Proof.
+      split. now rewrite LS_iff_DDC_BDP_BEP_BCC.
+      split. intros (h1 & h2 & h3 & h4). repeat split; eauto; now apply res_BDC2.
+      split. intros (h1 & h2 & h3).
+      assert DDC as h4 by (now apply BDC2_impl_DDC).
+      assert BCC. apply BDC_impl_BCC. now apply BDC2_impl_BDC.
+      assert DLS by now rewrite LS_iff_DDC_BDP_BEP_BCC.
+      now apply LS_impl_OBDC.
+      intro H. now apply LS_downward'.
+    Qed.
+  
 
 End LSiffDC.
